thy/LevelCollapse.thy
@@ -1,9 +1,24 @@
+section{* Collapsing the levels *}
 theory LevelCollapse
 imports Conc_Impl
 begin
+text{* 
+The theory up to this point is implemented in a way that separated the different aspects into different levels.
+This is highly beneficial for us, since it allows us to tackle the difficulties arising in small chunks.
+However, exporting this to the user would be highly impractical.
+Thus, this theory collapses all the different levels (i.e. refinement steps) and relates the computations in the heap monad to 
+@{type boolfunc}.
+*}
 
 definition "bddmi_rel cs \<equiv> {(a,c)|a b c. (a,b) \<in> bf_ifex_rel \<and> (c,b) \<in> Rmi cs}"
 definition "bdd_relator p s \<equiv> \<exists>\<^sub>Acs. is_bdd_impl cs s * \<up>(p \<subseteq> (bddmi_rel cs) \<and> bdd_sane cs)"
+
+text{*
+The @{type assn} predicate @{term bdd_relator} is the interface that is exposed to the user.
+(The contents of the definition are not exposed.)
+*}
+
+lemma bdd_relator_mono: "q \<subseteq> p \<Longrightarrow> bdd_relator p s \<Longrightarrow>\<^sub>A bdd_relator q s" unfolding bdd_relator_def by sep_auto
 
 thm bdd_relator_def[unfolded bddmi_rel_def, simplified]
 lemma join_hlp1: "is_bdd_impl a s * is_bdd_impl b s \<Longrightarrow>\<^sub>A is_bdd_impl a s * is_bdd_impl b s * \<up>(a = b)"
@@ -47,8 +62,7 @@ lemma add_true:
 	using assms add_anything[where x=true] by force
 
 thm iteci_rule[THEN mp] brofix.ite_impl_R ifex_ite_rel_bf
-(* Yeah, this is rubbish. *)
-lemma "
+lemma iteci_rule[sep_heap_rules]: "
 \<lbrakk>(ib, ic) \<in> rp; (tb, tc) \<in> rp; (eb, ec) \<in> rp\<rbrakk> \<Longrightarrow>
 <bdd_relator rp s> 
 	iteci ic tc ec s
@@ -82,6 +96,157 @@ lemma "
 	apply assumption
 done
 
+lemma tci_rule[sep_heap_rules]:
+"<bdd_relator rp s> 
+	tci s
+<\<lambda>(r,s'). bdd_relator (insert (bf_True,r) rp) s'>\<^sub>t"
+	apply(unfold bdd_relator_def)
+	apply(intro norm_pre_ex_rule)
+	apply(clarsimp)
+	apply(frule brofix.Timpl_rule)
+	apply(drule ospecD2)
+	apply(clarify)
+	apply(sep_auto)
+	 apply(unfold bddmi_rel_def)
+	 apply(clarsimp)
+	apply(force simp add: brofix.les_def)
+done
+
+lemma fci_rule[sep_heap_rules]:
+"<bdd_relator rp s> 
+	fci s
+<\<lambda>(r,s'). bdd_relator (insert (bf_False,r) rp) s'>\<^sub>t"
+	apply(unfold bdd_relator_def)
+	apply(intro norm_pre_ex_rule)
+	apply(clarsimp)
+	apply(frule brofix.Fimpl_rule)
+	apply(drule ospecD2)
+	apply(clarify)
+	apply(sep_auto)
+	 apply(unfold bddmi_rel_def)
+	 apply(clarsimp)
+	apply(force simp add: brofix.les_def)
+done
+
+text{* IFC/ifmi/ifci require that the variable order is ensured by the user. 
+Instead of using ifci, a combination of litci and iteci have to be used. *}
+lemma [sep_heap_rules]:
+"\<lbrakk>(tb, tc) \<in> rp; (eb, ec) \<in> rp\<rbrakk> \<Longrightarrow>
+<bdd_relator rp s> 
+	ifci v tc ec s
+<\<lambda>(r,s'). bdd_relator (insert (bf_if v tb eb,r) rp) s'>\<^sub>t"
+(*
+	apply(unfold bdd_relator_def)
+	apply(intro norm_pre_ex_rule)
+	apply(unfold bddmi_rel_def)
+	apply(clarsimp)
+	apply(drule (1) rev_subsetD)+
+	apply(clarsimp)
+	apply(frule (2) brofix.IFimpl_rule[of _ tc _ ec])
+	apply(drule ospecD2)
+	apply(clarify)
+	apply(sep_auto)
+	
+	 apply(unfold bddmi_rel_def)
+	 apply(clarsimp)
+	 apply(rule_tac x = Falseif in exI) (* okay, now I'm starting to prove something new, which I shouldn't *)
+	 apply(auto simp add: bf_False_def bf_ifex_rel_def)[1]
+	apply(force sim p add: brofix.les_def)*)
+oops
+lemma notci_rule[sep_heap_rules]:
+	assumes "(tb, tc) \<in> rp"
+	shows "<bdd_relator rp s> notci tc s <\<lambda>(r,s'). bdd_relator (insert (bf_not tb,r) rp) s'>\<^sub>t"
+using assms
+	apply(unfold bf_not_def notci_def)
+	apply(rule bind_rule, rule fci_rule, clarify)
+	apply(rule bind_rule, rule tci_rule[THEN add_true], clarify)
+	apply(rule cons_post_rule)
+	apply(rule iteci_rule[THEN add_true]; blast)
+	apply(rule fr_refl)
+	apply(clarify)
+	apply(rule bdd_relator_mono; fast)
+done
+
+lemma cirules1[sep_heap_rules]:
+	assumes "(tb, tc) \<in> rp" "(eb, ec) \<in> rp"
+	shows
+		"<bdd_relator rp s> andci tc ec s <\<lambda>(r,s'). bdd_relator (insert (bf_and tb eb,r) rp) s'>\<^sub>t"
+		"<bdd_relator rp s> orci tc ec s <\<lambda>(r,s'). bdd_relator (insert (bf_or tb eb,r) rp) s'>\<^sub>t"
+		"<bdd_relator rp s> biimpci tc ec s <\<lambda>(r,s'). bdd_relator (insert (bf_biimp tb eb,r) rp) s'>\<^sub>t"
+		"<bdd_relator rp s> xorci tc ec s <\<lambda>(r,s'). bdd_relator (insert (bf_xor tb eb,r) rp) s'>\<^sub>t"
+(* actually, these functions would allow for more insert. I think that would be inconvenient though. *)
+using assms
+by(unfold bf_and_def andci_def bf_or_def orci_def bf_nand_def biimpci_def bf_biimp_def xorci_def bf_xor_alt)
+  (rule bind_rule, (rule fci_rule | rule tci_rule | (rule notci_rule; assumption)); clarify, rule cons_post_rule, (rule iteci_rule[THEN add_true]; blast), 
+	rule fr_refl; clarify, (rule bdd_relator_mono; fast))+
+(* Because I can, that's why. (see below for the unfolded version) *)
+
+lemma cirules2[sep_heap_rules]:
+	assumes "(tb, tc) \<in> rp" "(eb, ec) \<in> rp"
+	shows
+		"<bdd_relator rp s> nandci tc ec s <\<lambda>(r,s'). bdd_relator (insert (bf_nand tb eb,r) rp) s'>\<^sub>t"
+		"<bdd_relator rp s> norci tc ec s <\<lambda>(r,s'). bdd_relator (insert (bf_nor tb eb,r) rp) s'>\<^sub>t"
+	using assms
+	by(sep_auto intro!: fr_refl bdd_relator_mono simp: nandci_def bf_nand_def norci_def bf_nor_def)+
+(* in case sep_auto starts acting up here like it does in the proof above:
+apply(rule bind_rule)
+apply(rule cirules1(2,1); assumption)
+apply(clarify)
+apply(rule cons_post_rule)
+apply(rule notci_rule[THEN add_true]; blast)
+apply(rule fr_refl)
+apply(clarify)
+apply(rule bdd_relator_mono)
+apply(fast)
+*)
+
+lemma litci_rule[sep_heap_rules]:
+	"<bdd_relator rp s> litci v s <\<lambda>(r,s'). bdd_relator (insert (bf_lit v,r) rp) s'>\<^sub>t"
+using assms
+	apply(unfold litci_def)
+	apply(subgoal_tac "\<And>t ab bb.
+		   <bdd_relator (insert (bf_False, ab) (insert (bf_True, t) rp)) bb *
+			true> ifci v t ab bb <\<lambda>r. case r of (r, x) \<Rightarrow> bdd_relator (insert (bf_lit v, r) rp) x>\<^sub>t")
+	 apply(sep_auto; fail)
+	apply(rename_tac tc fc sc)
+	apply(unfold bdd_relator_def[abs_def])
+	apply(clarsimp)
+	apply(intro norm_pre_ex_rule)
+	apply(clarsimp)
+	apply(unfold bddmi_rel_def)
+	apply(clarsimp simp only: bf_ifex_rel_consts_ensured)
+	apply(rename_tac tc fc sc sm a aa b ba fm tm)
+	apply(frule_tac brofix.IFimpl_rule)
+	  apply(thin_tac "(fm, Falseif) \<in> Rmi sm") apply(assumption) apply(assumption) (* sorry for the hacky hack, I don't know how to instantiate IFimpl_rule *)
+	apply(clarsimp)
+	apply(drule ospecD2)
+	apply(clarify)
+	apply(sep_auto)
+	apply(force simp add: brofix.les_def)
+done
+
+lemma tautci_rule[sep_heap_rules]:
+	shows "(tb, tc) \<in> rp \<Longrightarrow> <bdd_relator rp s> tautci tc s <\<lambda>r. bdd_relator rp s * \<up>(r \<longleftrightarrow> tb = bf_True)>\<^sub>t"
+	apply(unfold tautci_def)
+	apply(unfold bdd_relator_def)
+	apply(intro norm_pre_ex_rule; clarsimp)
+	apply(unfold bddmi_rel_def)
+	apply(drule (1) rev_subsetD)
+	apply(clarsimp)
+	apply(rename_tac sm ti)
+	apply(case_tac ti; clarify; frule (1) brofix.DESTRimpl_rules; drule ospecD2; clarify)
+	  apply(sep_auto; fail)
+	 apply(sep_auto; simp add: bf_False_def bf_True_def fun_eq_iff; fail)
+	apply(sep_auto)
+done
+
+lemma emptyci_rule[sep_heap_rules]:
+	shows "<emp> emptyci <\<lambda>r. bdd_relator {} r>\<^sub>t"
+by(sep_auto simp: bdd_relator_def)
+
+(* At some point in history, I've got to make sure that all those emptyci_rule and firends don't appear duplicate.
+   Today is not this day. *)
+
 (* I had some nice code_printing setup here, to implement blita/blit'. But that only did what would have been generated anyway *)
 lemma [code del]:
     "blit src si dst di len
@@ -89,7 +254,7 @@ lemma [code del]:
           (integer_of_nat len)" by (simp add: blit'_def)
 declare blit_def[code]
 
-(* Todo: Verify all of these\<dots>, except graphifyci *)
+(* Todo: verify iteci_opt *)
 export_code open iteci_opt iteci notci andci orci nandci norci biimpci xorci ifci tci fci tautci emptyci graphifyci litci in Haskell module_name IBDD file "../hs/gen"
   
 (* value "do { e \<leftarrow> emptyci; (graphifyci ''asdf'' 1 e) }" hm. *)
